Contracts.thy
@@ -1,0 +1,336 @@
+theory Contracts
+imports SeparationLogic
+begin
+
+fun strip_prenex :: "form \<Rightarrow> (var set \<times> form)" where
+  "strip_prenex (Exists x f) = (let (vs,f') = strip_prenex f in (insert x vs,f'))"
+| "strip_prenex f = ({},f)"
+
+fun simplify_emp_sepconj :: "form \<Rightarrow> form" where
+  "simplify_emp_sepconj (f1 \<^emph> f2) = 
+  (case simplify_emp_sepconj f1 of Emp \<Rightarrow> simplify_emp_sepconj f2 
+  | f1' \<Rightarrow> (case simplify_emp_sepconj f2 of Emp \<Rightarrow> f1' 
+  | f2' \<Rightarrow> f1' \<^emph> f2'))"
+| "simplify_emp_sepconj (Disj f1 f2) = Disj (simplify_emp_sepconj f1) (simplify_emp_sepconj f2)"
+| "simplify_emp_sepconj (Exists v f) = Exists v (simplify_emp_sepconj f)"
+| "simplify_emp_sepconj P = P"
+
+lemma simplification_sound: "separation_logic.form_semantics \<Lambda> d\<Lambda> (S,B,M) (simplify_emp_sepconj P) =
+  separation_logic.form_semantics \<Lambda> d\<Lambda> (S,B,M) P" (is "?sem (S,B,M) (_ P) = ?sem (S,B,M) P")
+proof
+assume "?sem (S, B, M) (simplify_emp_sepconj P)"
+then show "?sem (S, B, M) P" proof (induction P arbitrary: S B M)
+  case (SepConj P1 P2)
+  then show ?case proof (cases "simplify_emp_sepconj P1=Emp")
+    case True
+    then have "?sem (S,B,Map.empty) (simplify_emp_sepconj P1)" 
+      by (auto simp: separation_logic.form_semantics.simps)
+    with SepConj have "?sem (S,B,Map.empty) P1" by simp
+    moreover from True SepConj have "?sem (S,B,M) P2" by simp
+    ultimately show ?thesis by (auto simp: separation_logic.form_semantics.simps) fastforce
+  next
+    case False
+    then have P1: "simplify_emp_sepconj P1 \<noteq> Emp" .
+    then show ?thesis proof (cases "simplify_emp_sepconj P2=Emp")
+      case True
+      then have "?sem (S,B,Map.empty) (simplify_emp_sepconj P2)" 
+        by (auto simp: separation_logic.form_semantics.simps)
+      with SepConj have P2: "?sem (S,B,Map.empty) P2" by simp
+      from True P1 have "simplify_emp_sepconj (P1 \<^emph> P2) = simplify_emp_sepconj P1"
+        by (auto split: form.splits)
+      with SepConj have "?sem (S,B,M) P1" by simp
+      with P2 show ?thesis by (auto simp: separation_logic.form_semantics.simps) fastforce
+    next
+      case False
+      with P1 have "simplify_emp_sepconj (P1 \<^emph> P2) = ((simplify_emp_sepconj P1) 
+        \<^emph> (simplify_emp_sepconj P2))" by (auto split: form.splits)
+      from SepConj(3)[unfolded this] obtain M1 M2 where M: "dom M1 \<inter> dom M2 = {}" "M = M1 ++ M2" 
+        "?sem (S,B,M1) (simplify_emp_sepconj P1)" "?sem (S,B,M2) (simplify_emp_sepconj P2)"
+        unfolding separation_logic.form_semantics.simps by auto
+      with SepConj have "?sem (S,B,M1) P1" "?sem (S,B,M2) P2" by simp_all
+      with M show ?thesis by (auto simp: separation_logic.form_semantics.simps)
+    qed
+  qed    
+next
+  case (Disj P1 P2)
+  then have "?sem (S,B,M) ((simplify_emp_sepconj P1) \<or>\<^sub>s (simplify_emp_sepconj P2))"
+    by simp
+  then have "(?sem (S,B,M) (simplify_emp_sepconj P1) \<or> ?sem (S,B,M) (simplify_emp_sepconj P2))" 
+    unfolding separation_logic.form_semantics.simps(5) .
+  with Disj(1,2) show ?case unfolding separation_logic.form_semantics.simps(5) by auto
+next
+  case (Exists x1 P)
+  then have "?sem (S, B, M) (Exists x1 (simplify_emp_sepconj P))" by simp
+  then have "\<exists>v. ?sem (update_stack S x1 v,B,M) (simplify_emp_sepconj P)"
+    unfolding separation_logic.form_semantics.simps(9) .
+  with Exists(1) show ?case unfolding separation_logic.form_semantics.simps(9) by auto
+qed (simp_all)
+next
+assume "?sem (S, B, M) P"
+then show "?sem (S, B, M) (simplify_emp_sepconj P)" proof (induction P arbitrary: S B M)
+  case (SepConj P1 P2)
+  then obtain M1 M2 where M: "dom M1 \<inter> dom M2 = {}" "M = M1 ++ M2" "?sem (S,B,M1) P1" "?sem (S,B,M2) P2"
+    by (auto simp: separation_logic.form_semantics.simps)
+  then show ?case proof (cases "simplify_emp_sepconj P1=Emp")
+    case True
+    with SepConj(1)[OF M(3)] have "M1 = Map.empty" by (auto simp: separation_logic.form_semantics.simps)
+    with M(2) have "M=M2" by simp
+    with M(4) SepConj(2) have "?sem (S,B,M) (simplify_emp_sepconj P2)" by simp
+    with True show ?thesis by simp
+  next
+    case False
+    then have P1: "simplify_emp_sepconj P1 \<noteq> Emp" .
+    then show ?thesis proof (cases "simplify_emp_sepconj P2=Emp")
+      case True
+      with SepConj(2)[OF M(4)] have "M2 = Map.empty" by (auto simp: separation_logic.form_semantics.simps)
+      with M(2) have "M=M1" by simp
+      with M(3) SepConj(1) have "?sem (S,B,M) (simplify_emp_sepconj P1)" by simp
+      moreover from P1 True have "simplify_emp_sepconj (P1 \<^emph> P2) = simplify_emp_sepconj P1" 
+        by (auto split: form.splits)
+      ultimately show ?thesis by simp
+    next
+      case False
+      from M SepConj have "?sem (S,B,M1) (simplify_emp_sepconj P1)" "?sem (S,B,M2) (simplify_emp_sepconj P2)"
+        by auto
+      moreover from False P1 have "simplify_emp_sepconj (P1 \<^emph> P2) = ((simplify_emp_sepconj P1) 
+        \<^emph> (simplify_emp_sepconj P2))" by (auto split: form.splits)
+      ultimately show ?thesis using M(1,2) by (auto simp: separation_logic.form_semantics.simps)
+    qed
+  qed
+next
+  case (Disj P1 P2)
+  then show ?case by (auto simp: separation_logic.form_semantics.simps(5))
+next
+  case (Exists x1 P)
+  then show ?case by (auto simp: separation_logic.form_semantics.simps(9))
+qed (simp_all)
+qed
+
+context separation_logic begin
+abbreviation star_disj :: "form list \<Rightarrow> form" where
+  "star_disj Q \<equiv> fold (\<or>\<^sub>s) Q FalseF" 
+end
+
+text \<open>The paper distinguishes program variables and logical variables.
+  For the formalization, it suffices to know the arguments to a function 
+  to get the program variables, as the function can't use any other variables.
+  Therefore, we do not use different types for these two kinds of variables but just different sets.
+  We also use meta-variables wherever possible.\<close>
+ 
+type_synonym pre_contract = "(form\<times>(form list)) set"
+
+value "simplify_emp_sepconj (foldr (\<lambda>(x,e) r. (f_eq x e) \<^emph> r) (zip [x,y] [X,Y]) Emp)"
+
+typedef contract = "{(cs, (f,args))::pre_contract\<times>func | cs args f.
+  \<forall>(P,Q)\<in>cs. quantifier_free P \<and> symbolic_heap P \<and> \<comment> \<open>P is a quantifier-free symbolic heap\<close>
+  \<comment> \<open>Q is a disjunction of single formulas of the form \<open>\<exists>UQ. Qf \<^emph> Qeq\<close>\<close>
+  list_all (\<lambda>q. case strip_prenex q of (UQ, Qf \<^emph> Qeq) \<Rightarrow>
+    \<comment> \<open>The prenex variables are the logical ones in Qf and Qeq, that are not also in P.\<close>
+    UQ = (free_vars Qf \<union> free_vars Qeq) - set args - free_vars P \<and>
+    \<comment> \<open>Qf is a quantifier-free symbolic heap with only logical variables\<close>
+    quantifier_free Qf \<and> symbolic_heap Qf \<and> free_vars Qf \<inter> set args = {} \<and>
+    \<comment> \<open>Qeq is of the form \<open>x1=e1 \<^emph> ... \<^emph> xn=en \<^emph> Emp\<close> for arguments xi and some expressions e 
+      that only contain logical variables.\<close>
+    (\<exists>eqs. Qeq = simplify_emp_sepconj (foldr (\<lambda>(x, e). (\<^emph>) (f_eq x e)) (zip args eqs) Emp)
+    \<and> list_all (\<lambda>e. free_vars e \<inter> set args = {}) eqs)
+    | _ \<Rightarrow> False) Q}" by auto
+
+setup_lifting type_definition_contract
+
+context program_logic
+begin
+lift_definition sound :: "contract \<Rightarrow> bool" is
+  "\<lambda>(cs, (f,args)). \<forall>(P,Qs) \<in> cs. \<forall>c c' F.
+    (((c \<turnstile> (P\<^emph>F)) \<and> fun_semantics fs f c c' \<and> symbolic_heap F \<and> free_vars F \<inter> set args = {}) 
+    \<longrightarrow> (c' \<turnstile> ((star_disj Qs) \<^emph> F)))" .
+end
+
+abbreviation single_stmt_cfg :: "func \<Rightarrow> command \<Rightarrow> cfg" where
+  "single_stmt_cfg f cmd \<equiv> (f, {(entry,cmd,exit)})"
+
+abbreviation single_fun_prog :: "func \<Rightarrow> command \<Rightarrow> prog" where
+  "single_fun_prog f cmd \<equiv> (case f of (n,args) \<Rightarrow> [n\<mapsto>single_stmt_cfg f cmd])"
+
+locale standard_prog = fixes x y z X Y Z u :: var 
+  assumes var_sep: "{x,y,z,u} \<inter> {X,Y,Z} = {}" and diff_var: "x\<noteq>y\<and>y\<noteq>z\<and>x\<noteq>z\<and>x\<noteq>u\<and>y\<noteq>u\<and>z\<noteq>u"
+begin
+
+definition assign :: prog where "assign \<equiv> single_fun_prog (''assign'',[x,y]) (AssignVar x y)"
+definition assign_contract :: pre_contract where 
+  "assign_contract \<equiv> {(f_eq y Y,[Emp \<^emph> (f_eq x Y)\<^emph>(f_eq y Y)])}"
+lift_definition assign_c :: contract is "(assign_contract, (''assign'',[x,y]))"
+proof (auto simp: assign_contract_def)
+  define eqs where "eqs = [VarE Y,VarE Y]"
+  then have "(f_eq x Y \<^emph> f_eq y Y) = simplify_emp_sepconj (foldr (\<lambda>(x, e). (\<^emph>) (f_eq x e)) (zip [x, y] eqs) Emp) 
+    \<and> list_all (\<lambda>e. x \<notin> free_vars e \<and> y \<notin> free_vars e) eqs"
+    using var_sep eqs_def by auto
+  then show "\<exists>eqs. (f_eq x Y \<^emph> f_eq y Y) = simplify_emp_sepconj (foldr (\<lambda>(x, e). (\<^emph>) (f_eq x e)) (zip [x, y] eqs) Emp) 
+    \<and> list_all (\<lambda>e. x \<notin> free_vars e \<and> y \<notin> free_vars e) eqs" by auto
+qed
+
+definition const :: "val \<Rightarrow> prog" where "const k \<equiv> single_fun_prog (''const'',[x]) (AssignConst x k)"
+definition const_contract :: "val \<Rightarrow> pre_contract" where 
+  "const_contract k \<equiv> {(Emp,[Emp \<^emph> (f_eq x k)])}"
+lift_definition const_c :: "val \<Rightarrow> contract" is "\<lambda>k. (const_contract k, (''const'',[x]))"
+proof (auto simp: const_contract_def)
+  fix k :: val
+  define eqs where "eqs = [ConstE k]"
+  then have "(f_eq x (ConstE k)) = simplify_emp_sepconj (foldr (\<lambda>(x, e). (\<^emph>) (f_eq x e)) (zip [x] eqs) Emp) 
+    \<and> list_all (\<lambda>e. x \<notin> free_vars e) eqs"
+    using var_sep eqs_def by auto
+  then show "\<exists>eqs. (f_eq x (ConstE k)) = simplify_emp_sepconj (foldr (\<lambda>(x, e). (\<^emph>) (f_eq x e)) (zip [x] eqs) Emp) 
+    \<and> list_all (\<lambda>e. x \<notin> free_vars e) eqs" by auto
+qed
+
+definition load :: prog where "load \<equiv> single_fun_prog (''load'',[x,y]) (Load x y)"
+definition load_contract :: pre_contract where 
+  "load_contract \<equiv> {((f_eq y Y)\<^emph>(Y\<mapsto>\<^sub>sz),[(Y\<mapsto>\<^sub>sz) \<^emph> (f_eq x z)\<^emph>(f_eq y Y)])}"
+lift_definition load_c :: contract is "(load_contract, (''load'',[x,y]))"
+  using var_sep[simplified]
+proof (auto simp: load_contract_def diff_var)
+  define eqs where "eqs = [VarE z, Y]"
+  then have "(f_eq x z \<^emph> f_eq y Y) = simplify_emp_sepconj (foldr (\<lambda>(x, e). (\<^emph>) (f_eq x e)) (zip [x,y] eqs) Emp) 
+    \<and> list_all (\<lambda>e. x \<notin> free_vars e \<and> y \<notin> free_vars e) eqs"
+    using eqs_def var_sep diff_var by auto
+  then show "\<exists>eqs. (f_eq x z \<^emph> f_eq y Y) = simplify_emp_sepconj (foldr (\<lambda>(x, e). (\<^emph>) (f_eq x e)) (zip [x,y] eqs) Emp) 
+    \<and> list_all (\<lambda>e. x \<notin> free_vars e \<and> y \<notin> free_vars e) eqs" by auto
+qed
+
+definition store :: prog where "store \<equiv> single_fun_prog (''store'',[x,y]) (Store x y)"
+definition store_contract :: pre_contract where 
+  "store_contract \<equiv> {((f_eq x X)\<^emph>(f_eq y Y)\<^emph>(X\<mapsto>\<^sub>sz),[(X\<mapsto>\<^sub>sY) \<^emph> (f_eq x X)\<^emph>(f_eq y Y)])}"
+lift_definition store_c :: contract is "(store_contract, (''store'',[x,y]))"
+  using var_sep[simplified]
+proof (auto simp: store_contract_def)
+  define eqs where "eqs = [VarE X, Y]"
+  then have "(f_eq x X \<^emph> f_eq y Y) = simplify_emp_sepconj (foldr (\<lambda>(x, e). (\<^emph>) (f_eq x e)) (zip [x,y] eqs) Emp) 
+    \<and> list_all (\<lambda>e. x \<notin> free_vars e \<and> y \<notin> free_vars e) eqs"
+    using eqs_def var_sep diff_var by auto
+  then show "\<exists>eqs. (f_eq x X \<^emph> f_eq y Y) = simplify_emp_sepconj (foldr (\<lambda>(x, e). (\<^emph>) (f_eq x e)) (zip [x,y] eqs) Emp) 
+    \<and> list_all (\<lambda>e. x \<notin> free_vars e \<and> y \<notin> free_vars e) eqs" by auto
+qed
+
+definition malloc :: prog where "malloc \<equiv> single_fun_prog (''malloc'',[x,y]) (Malloc x y)"
+definition malloc_contract :: pre_contract where 
+  "malloc_contract \<equiv> {((f_eq y Y),
+    [Emp \<^emph> (f_eq x (null x))\<^emph>(f_eq y Y),
+    Exists u (((u\<mapsto>\<top>[Y])\<^emph>(f_eq (Base u) u)\<^emph>(f_eq (Ende u) (e_add u Y))) \<^emph> (f_eq x u)\<^emph>(f_eq y Y))])}"
+lift_definition malloc_c :: contract is "(malloc_contract, (''malloc'',[x,y]))"
+  using var_sep[simplified] diff_var
+proof (auto simp: malloc_contract_def)
+  define eqs where "eqs = [ConstE (null x), Y]"
+  then have "(f_eq x (null x) \<^emph> f_eq y Y) = simplify_emp_sepconj (foldr (\<lambda>(x, e). (\<^emph>) (f_eq (VarE x) e)) (zip [x,y] eqs) Emp) 
+    \<and> list_all (\<lambda>e. x \<notin> free_vars e \<and> y \<notin> free_vars e) eqs"
+    using eqs_def var_sep diff_var by auto
+  then show "\<exists>eqs. (f_eq x (null x) \<^emph> f_eq y Y) = simplify_emp_sepconj (foldr (\<lambda>(x, e). (\<^emph>) (f_eq (VarE x) e)) (zip [x,y] eqs) Emp) 
+    \<and> list_all (\<lambda>e. x \<notin> free_vars e \<and> y \<notin> free_vars e) eqs" by auto
+next
+  define eqs where "eqs = [VarE u, Y]"
+  then have "(f_eq x u \<^emph> f_eq y Y) = simplify_emp_sepconj (foldr (\<lambda>(x, e). (\<^emph>) (f_eq (VarE x) e)) (zip [x,y] eqs) Emp) 
+    \<and> list_all (\<lambda>e. x \<notin> free_vars e \<and> y \<notin> free_vars e) eqs"
+    using eqs_def var_sep diff_var by auto
+  then show "\<exists>eqs. (f_eq x u \<^emph> f_eq y Y) = simplify_emp_sepconj (foldr (\<lambda>(x, e). (\<^emph>) (f_eq (VarE x) e)) (zip [x,y] eqs) Emp) 
+    \<and> list_all (\<lambda>e. x \<notin> free_vars e \<and> y \<notin> free_vars e) eqs" by auto
+qed
+
+definition free :: prog where "free \<equiv> single_fun_prog (''free'',[x]) (Free x)"
+definition free_contract :: pre_contract where 
+  "free_contract \<equiv> {((f_eq x X)\<^emph>(X\<mapsto>\<top>[y])\<^emph>(f_eq (Base X) X)\<^emph>(f_eq (Ende X) (e_add X y)),[Emp \<^emph> (f_eq x X)])}"
+lift_definition free_c :: contract is "(free_contract, (''free'',[x]))"
+proof (auto simp: free_contract_def)
+  define eqs where "eqs = [VarE X]"
+  then have "f_eq x X = simplify_emp_sepconj (foldr (\<lambda>(x, e). (\<^emph>) (f_eq x e)) (zip [x] eqs) Emp) 
+    \<and> list_all (\<lambda>e. x \<notin> free_vars e) eqs"
+    using eqs_def var_sep diff_var by auto
+  then show "\<exists>eqs. f_eq x X = simplify_emp_sepconj (foldr (\<lambda>(x, e). (\<^emph>) (f_eq x e)) (zip [x] eqs) Emp) 
+    \<and> list_all (\<lambda>e. x \<notin> free_vars e) eqs" by auto
+qed
+
+definition assign_binop :: "binop \<Rightarrow> prog" where "assign_binop op \<equiv> 
+  single_fun_prog (''assign_binop'',[x,y,z]) (BinOp op x y z)"
+definition binop_contract :: "binop \<Rightarrow> pre_contract" where 
+  "binop_contract op \<equiv> {((f_eq y Y)\<^emph>(f_eq z Z),[Emp \<^emph> (f_eq x (BinOpE op Y Z))\<^emph>(f_eq y Y)\<^emph>(f_eq z Z)])}"
+lift_definition binop_c :: "binop \<Rightarrow> contract" is "\<lambda>op. (binop_contract op, (''assign_binop'',[x,y,z]))"
+proof (auto simp: binop_contract_def)
+  fix op :: binop
+  define eqs where "eqs = [BinOpE op Y Z,Y,Z]"
+  then have "f_eq x (BinOpE op Y Z)\<^emph>f_eq y Y\<^emph>f_eq z Z = simplify_emp_sepconj (foldr (\<lambda>(x, e). (\<^emph>) (f_eq x e)) (zip [x,y,z] eqs) Emp) 
+    \<and> list_all (\<lambda>e. x \<notin> free_vars e \<and> y \<notin> free_vars e \<and> z \<notin> free_vars e) eqs"
+    using eqs_def var_sep diff_var by auto
+  then show "\<exists>eqs. f_eq x (BinOpE op Y Z)\<^emph>f_eq y Y\<^emph>f_eq z Z = simplify_emp_sepconj (foldr (\<lambda>(x, e). (\<^emph>) (f_eq x e)) (zip [x,y,z] eqs) Emp) 
+    \<and> list_all (\<lambda>e. x \<notin> free_vars e \<and> y \<notin> free_vars e \<and> z \<notin> free_vars e) eqs" by auto
+qed
+
+definition assign_unop ::  "unop \<Rightarrow> prog" where "assign_unop op \<equiv> 
+  single_fun_prog (''assign_unop'',[x,y]) (UnOp op x y)"
+definition unop_contract :: "unop \<Rightarrow> pre_contract" where 
+  "unop_contract op \<equiv> {((f_eq y Y),[Emp \<^emph> (f_eq x (UnOpE op Y))\<^emph>(f_eq y Y)])}"
+lift_definition unop_c :: "unop \<Rightarrow> contract" is "\<lambda>op. (unop_contract op, (''assign_unop'',[x,y]))"
+proof (auto simp: unop_contract_def)
+  fix op :: unop
+  define eqs where "eqs = [UnOpE op Y,Y]"
+  then have "f_eq x (UnOpE op Y)\<^emph>f_eq y Y = simplify_emp_sepconj (foldr (\<lambda>(x, e). (\<^emph>) (f_eq x e)) (zip [x,y] eqs) Emp) 
+    \<and> list_all (\<lambda>e. x \<notin> free_vars e \<and> y \<notin> free_vars e) eqs"
+    using eqs_def var_sep diff_var by auto
+  then show "\<exists>eqs. f_eq x (UnOpE op Y)\<^emph>f_eq y Y = simplify_emp_sepconj (foldr (\<lambda>(x, e). (\<^emph>) (f_eq x e)) (zip [x,y] eqs) Emp) 
+    \<and> list_all (\<lambda>e. x \<notin> free_vars e \<and> y \<notin> free_vars e) eqs" by auto
+qed
+
+definition ptrplus :: prog where "ptrplus \<equiv> single_fun_prog (''ptrplus'',[x,y,z]) (PtrPlus x y z)"
+abbreviation "ptrplus\<phi> \<equiv> (Atom Neq (Base Y) null_loc)\<^emph>(f_eq (Base Y) (Base (e_add Y Z)))\<^emph>
+  (f_eq (Ende Y) (Ende (e_add Y Z)))"
+abbreviation "ptrplus\<phi>2 \<equiv> (Atom Neq (Base Y) null_loc)\<^emph>(f_eq (e_add Y Z) (Ende Y))"
+definition ptrplus_contract :: pre_contract where 
+  "ptrplus_contract \<equiv> {
+  ((f_eq y Y)\<^emph>(f_eq z Z)\<^emph>ptrplus\<phi>,[ptrplus\<phi> \<^emph> (f_eq x (e_add Y Z))\<^emph>(f_eq y Y)\<^emph>(f_eq z Z)]),
+  ((f_eq y Y)\<^emph>(f_eq z Z)\<^emph>ptrplus\<phi>2,[ptrplus\<phi>2 \<^emph> (f_eq x (e_add Y Z))\<^emph>(f_eq y Y)\<^emph>(f_eq z Z)])
+  }"
+lift_definition ptrplus_c :: contract is "(ptrplus_contract, (''ptrplus'',[x,y,z]))"
+  using var_sep[simplified] diff_var
+proof (auto simp: ptrplus_contract_def)
+  fix op :: unop
+  define eqs where "eqs = [e_add Y Z,Y,Z]"
+  then have "f_eq x (e_add Y Z)\<^emph>f_eq y Y\<^emph>f_eq z Z = simplify_emp_sepconj (foldr (\<lambda>(x, e). (\<^emph>) (f_eq x e)) (zip [x,y,z] eqs) Emp) 
+    \<and> list_all (\<lambda>e. x \<notin> free_vars e \<and> y \<notin> free_vars e \<and> z \<notin> free_vars e) eqs"
+    using eqs_def var_sep diff_var by auto
+  then show "\<exists>eqs. f_eq x (e_add Y Z)\<^emph>f_eq y Y\<^emph>f_eq z Z = simplify_emp_sepconj (foldr (\<lambda>(x, e). (\<^emph>) (f_eq x e)) (zip [x,y,z] eqs) Emp) 
+    \<and> list_all (\<lambda>e. x \<notin> free_vars e \<and> y \<notin> free_vars e \<and> z \<notin> free_vars e) eqs" by auto
+  then show "\<exists>eqs. f_eq x (e_add Y Z)\<^emph>f_eq y Y\<^emph>f_eq z Z = simplify_emp_sepconj (foldr (\<lambda>(x, e). (\<^emph>) (f_eq x e)) (zip [x,y,z] eqs) Emp) 
+    \<and> list_all (\<lambda>e. x \<notin> free_vars e \<and> y \<notin> free_vars e \<and> z \<notin> free_vars e) eqs" by auto
+qed
+
+definition ptrsub :: prog where "ptrsub \<equiv> single_fun_prog (''ptrsub'',[x,y,z]) (PtrSub x y z)"
+definition ptrsub_contract :: pre_contract where 
+  "ptrsub_contract \<equiv> {((f_eq y Y)\<^emph>(f_eq z Z)\<^emph>(Atom Neq (Base Y) null_loc)\<^emph>(Atom Leq (Base Y) Z)\<^emph>(Atom Leq Z (Ende Y)),
+  [Emp \<^emph> (f_eq x (BinOpE minus Y Z)\<^emph>(f_eq y Y)\<^emph>(f_eq z Z))])}"
+lift_definition ptrsubs_c :: contract is "(ptrsub_contract, (''ptrsub'',[x,y,z]))"
+proof (auto simp: ptrsub_contract_def)
+  fix op :: unop
+  define eqs where "eqs = [BinOpE Semantics.minus Y Z,Y,Z]"
+  then have "f_eq x (BinOpE Semantics.minus Y Z)\<^emph>f_eq y Y\<^emph>f_eq z Z = simplify_emp_sepconj (foldr (\<lambda>(x, e). (\<^emph>) (f_eq x e)) (zip [x,y,z] eqs) Emp) 
+    \<and> list_all (\<lambda>e. x \<notin> free_vars e \<and> y \<notin> free_vars e \<and> z \<notin> free_vars e) eqs"
+    using eqs_def var_sep diff_var by auto
+  then show "\<exists>eqs. f_eq x (BinOpE Semantics.minus Y Z)\<^emph>f_eq y Y\<^emph>f_eq z Z = simplify_emp_sepconj (foldr (\<lambda>(x, e). (\<^emph>) (f_eq x e)) (zip [x,y,z] eqs) Emp) 
+    \<and> list_all (\<lambda>e. x \<notin> free_vars e \<and> y \<notin> free_vars e \<and> z \<notin> free_vars e) eqs" by auto
+qed
+
+definition memcpy :: prog where "memcpy \<equiv> single_fun_prog (''memcpy'',[x,y,z]) (Memcpy x y z)"
+
+text \<open>The contracts for assume and assert don't follow the scheme, as the atomic conditions can't be 
+  part of either Qf (it can't talk about program variables) or Qeq (it already contains all equalities.\<close>
+definition assume_f :: "condition \<Rightarrow> prog" where "assume_f c \<equiv> single_fun_prog (''assume'',[y,z]) (Assume c y z)"
+definition assume_contract :: "condition \<Rightarrow> pre_contract" where 
+  "assume_contract c \<equiv> {((f_eq y Y)\<^emph>(f_eq z Z),[Atom c y z \<^emph> (f_eq y Y)\<^emph>(f_eq z Z)])}"
+lift_definition assume_c :: "condition \<Rightarrow> contract" is "\<lambda>c. (assume_contract c, (''assume'',[y,z]))"
+  oops
+
+definition assert_f :: "condition \<Rightarrow> prog" where "assert_f c \<equiv> single_fun_prog (''assert'',[x,y]) (Assert c x y)"
+definition assert_contract :: "condition \<Rightarrow> pre_contract" where 
+  "assert_contract c \<equiv> {(Atom c y z\<^emph>(f_eq y Y)\<^emph>(f_eq z Z),[Atom c y z \<^emph> (f_eq y Y)\<^emph>(f_eq z Z)])}"
+lift_definition assert_c :: "condition \<Rightarrow> contract" is "\<lambda>c. (assert_contract c, (''assert'',[y,z]))"
+  oops
+
+definition standard_prog :: prog where "standard_prog \<equiv> assign++load++store++malloc++free
+  ++ptrplus++ptrsub++memcpy"
+end
+end
